src/inClassNotes/final/var_test.lean
@@ -9,3 +9,7 @@ def Z : var nat := var.mk 2
 def P : var bool := var.mk 0
 def Q : var bool := var.mk 1
 def R : var bool := var.mk 2
+
+-- test our var_eq function
+example : var_eq X X = tt := rfl
+example : var_eq X Y = ff := rfl
